implement first functions for linear array

Scratch.thy
@@ -1,5 +1,5 @@
 theory Scratch
-  imports Main "Separation_Logic_Imperative_HOL.Sep_Examples" "Deriving.Derive"
+  imports Main "Separation_Logic_Imperative_HOL.Sep_Main" "Deriving.Derive" "HOL-Library.Code_Target_Nat"
 begin
 
 (**
@@ -17,12 +17,114 @@ derive countable cell
 instance cell :: (heap) heap
    by standard
 
-type_synonym 'a la = "'a cell ref ref"
+type_synonym 'a la = "'a cell ref"
 
 
 datatype 'a la_node = LA_node nat 'a "'a la_node list" "'a cell ref"
 datatype 'a la_tree = LA_tree "'a list" "'a la_node list" "'a cell ref"
 
+definition fold_assn where
+  "fold_assn assns = fold (*) assns emp"
 
 fun la_node_assn where
-   "la_node_assn prev (LA_node i a succs p) = (p \<mapsto>\<^sub>r Upd i a prev) * (\<forall>n\<in>succs. la_node_assn p n)"
+   "la_node_assn prev (LA_node i a succs p) = (p \<mapsto>\<^sub>r Upd i a prev) * (fold_assn (map (la_node_assn p) succs))"
+
+fun la_tree_assn where
+  "la_tree_assn (LA_tree vals succs p) = (\<exists>\<^sub>A ap. (p \<mapsto>\<^sub>r Array ap) * (ap  \<mapsto>\<^sub>a vals) * (fold_assn (map (la_node_assn p) succs)))"
+
+no_notation Ref.update ("_ := _" 62)
+notation Ref.update ("_ :=\<^sub>R _" 62)
+
+fun node_to_map :: "'a list \<Rightarrow> 'a la_node \<Rightarrow> ('a cell ref \<rightharpoonup> 'a list)" where
+  "node_to_map vals (LA_node i a succs p) = (
+    let vals' = vals[i:= a] 
+    in [p \<mapsto> vals'] ++ fold (++) (map (node_to_map vals') succs) Map.empty
+  )"
+
+fun node_to_map' :: "'a list \<Rightarrow> 'a la_node \<Rightarrow> ('a cell ref * 'a list) list" where
+  "node_to_map' vals (LA_node i a succs p) = (
+    let vals' = vals[i:= a] 
+    in (p, vals') # concat (map (node_to_map' vals') succs)
+  )"
+
+fun refs_node where 
+  "refs_node (LA_node i a succs p) = p # concat (map refs_node succs)"
+
+definition invar_node :: "'a la_node \<Rightarrow> bool" where
+  "invar_node node = distinct (refs_node node)"
+
+fun tree_to_map' where
+  "tree_to_map' (LA_tree vals succs p) = (p, vals) # concat (map (node_to_map' vals) succs)"
+
+fun refs_tree where
+  "refs_tree (LA_tree vals succs p) = p # concat (map refs_node succs)"
+
+definition invar_tree :: "'a la_tree \<Rightarrow> bool" where
+  "invar_tree tree = distinct (refs_tree tree)"
+
+lemma "map fst (node_to_map' xs n) = refs_node n"
+  apply(induction n arbitrary: xs)
+  by(auto simp: Let_def map_concat intro!: arg_cong[where f = concat])
+
+find_theorems "map _ (concat _)"
+thm arg_cong[where f = concat]
+
+lemma node_to_map'_refs: "map fst (node_to_map' xs n) = refs_node n"
+  apply(induction xs n rule: node_to_map'.induct)
+  by(auto simp: Let_def map_concat intro!: arg_cong[where f = concat])
+
+lemma tree_to_map'_refs: "map fst (tree_to_map' t) = refs_tree t"
+  apply(cases t) 
+  by (auto simp: node_to_map'_refs map_concat intro!: arg_cong[where f = concat])
+
+find_consts "(_ * _) list \<Rightarrow> (_ \<Rightarrow> _ option)"
+find_theorems "map_of" "distinct"
+
+lemma "invar_tree t \<Longrightarrow> distinct (map fst (tree_to_map' t))"
+  by (simp add: invar_tree_def tree_to_map'_refs)
+
+definition la_rel where
+  "la_rel t xs p \<longleftrightarrow> map_of (tree_to_map' t) p = Some xs"
+
+definition array_to_la where
+  "array_to_la a = do {
+    ref (Array a)
+  }"
+
+lemma [simp]: "fold_assn [] = emp"
+  unfolding fold_assn_def
+  by auto
+
+find_theorems "_ \<Longrightarrow>\<^sub>A \<exists>\<^sub>A _. _"
+
+lemma array_to_la: "<a \<mapsto>\<^sub>a xs> array_to_la a <\<lambda>r. \<exists>\<^sub>At. la_tree_assn t * \<up>(la_rel t xs r)>"
+  unfolding array_to_la_def 
+  apply vcg
+  subgoal for r
+    apply(rule ent_ex_postI[where x = "LA_tree xs [] r"])
+    by(sep_auto simp: la_rel_def)
+  .
+
+partial_function (heap) foo :: "nat \<Rightarrow> nat Heap"  where
+  "foo n = do { 
+      r \<leftarrow> foo (n);
+      return (r + 1)
+  }"
+
+
+definition array_to_la' where
+  "array_to_la' n x = do {
+    a \<leftarrow> Array.new n x;
+    Array.upd 0 (42::nat) a;
+    array_to_la a
+  }"
+
+definition test where "test = do {
+  r \<leftarrow> array_to_la' 2 (5::nat);
+  return r
+}"
+
+ML_val \<open>@{code test} ()\<close>
+
+export_code test in SML_imp module_name foo
+
